Allow spec simulation steps under cfupd
Previously, we could only do a spec step with an ncfupd, since the invariant
storing the trace of the spec execution was in an ncinv. This has been fine for
previous examples, but the journal requires potentially finishing an Atomically
block during CommitWait if we learn the commit was made durable in the crash
condition.

This commit allows additional steps under a cfupd by transferring the spec
assert to a normal invariant when the crash happens.  Special tokens will be
needed to continue doing transitions at that point of a crash. For the journal
FFI, there is a token per address, and holding any one allows further steps.

src/goose_lang/ffi/jrnl_ffi.v
@@ -1,4 +1,4 @@
-From iris.algebra Require Import auth agree excl csum.
+From iris.algebra Require Import auth frac agree excl csum.
 From Perennial.algebra Require Import auth_map.
 From RecordUpdate Require Import RecordSet.
 
@@ -195,16 +195,19 @@ Class jrnlG Σ :=
     jrnlG_data_name: gname;
     jrnlG_kinds_inG :> inG Σ (agreeR (leibnizO (gmap blkno kind)));
     jrnlG_kinds_name: gname;
+    jrnlG_crash_toks_inG :> mapG Σ addr unit;
+    jrnlG_crash_toks_name: gname;
   }.
 
 Class jrnl_preG Σ :=
   { jrnlG_preG_open_inG :> inG Σ openR;
     jrnlG_preG_data_inG:> mapG Σ addr obj;
     jrnlG_preG_kinds_inG:> inG Σ (agreeR (leibnizO (gmap blkno kind)));
+    jrnlG_preG_crash_toks_inG:> mapG Σ addr unit;
   }.
 
 Definition jrnlΣ : gFunctors :=
-  #[GFunctor openR; mapΣ addr obj; GFunctor (agreeR (leibnizO (gmap blkno kind)))].
+  #[GFunctor openR; mapΣ addr obj; GFunctor (agreeR (leibnizO (gmap blkno kind))); mapΣ addr unit].
 
 Instance subG_jrnlG Σ: subG jrnlΣ Σ → jrnl_preG Σ.
 Proof. solve_inG. Qed.
@@ -213,12 +216,14 @@ Record jrnl_names :=
   { jrnl_names_open: gname;
     jrnl_names_data: gname;
     jrnl_names_kinds: gname;
+    jrnl_names_crash: gname;
   }.
 
 Definition jrnl_get_names {Σ} (jG: jrnlG Σ) :=
   {| jrnl_names_open := jrnlG_open_name;
      jrnl_names_data := jrnlG_data_name;
-     jrnl_names_kinds := jrnlG_kinds_name |}.
+     jrnl_names_kinds := jrnlG_kinds_name;
+     jrnl_names_crash := jrnlG_crash_toks_name |}.
 
 Definition jrnl_update {Σ} (jG: jrnlG Σ) (names: jrnl_names) :=
   {| jrnlG_open_inG := jrnlG_open_inG;
@@ -227,6 +232,8 @@ Definition jrnl_update {Σ} (jG: jrnlG Σ) (names: jrnl_names) :=
      jrnlG_data_name := (jrnl_names_data names);
      jrnlG_kinds_inG := jrnlG_kinds_inG;
      jrnlG_kinds_name := (jrnl_names_kinds names);
+     jrnlG_crash_toks_inG := jrnlG_crash_toks_inG;
+     jrnlG_crash_toks_name := (jrnl_names_crash names);
   |}.
 
 Definition jrnl_update_pre {Σ} (jG: jrnl_preG Σ) (names: jrnl_names) :=
@@ -236,6 +243,8 @@ Definition jrnl_update_pre {Σ} (jG: jrnl_preG Σ) (names: jrnl_names) :=
      jrnlG_data_name := (jrnl_names_data names);
      jrnlG_kinds_inG := jrnlG_preG_kinds_inG;
      jrnlG_kinds_name := (jrnl_names_kinds names);
+     jrnlG_crash_toks_inG := jrnlG_preG_crash_toks_inG;
+     jrnlG_crash_toks_name := (jrnl_names_crash names);
   |}.
 
 Definition jrnl_open {Σ} {lG :jrnlG Σ} :=
@@ -251,6 +260,8 @@ Definition jrnl_kinds_lb {Σ} {lG: jrnlG Σ} (σj : gmap blkno kind) : iProp Σ 
 Definition jrnl_mapsto {Σ} {lG: jrnlG Σ} a q v : iProp Σ :=
   ptsto_mut (jrnlG_data_name) a q v ∗
   (∃ σj,  ⌜ size_consistent_and_aligned a v σj ⌝ ∗ jrnl_kinds σj).
+Definition jrnl_crash_tok {Σ} {lG: jrnlG Σ} a : iProp Σ :=
+  ptsto_mut (jrnlG_crash_toks_name) a 1 tt.
 
 Section jrnl_interp.
   Existing Instances jrnl_op jrnl_model jrnl_val_ty.
@@ -266,8 +277,16 @@ Section jrnl_interp.
     | Closed s => jrnl_closed_auth ∗ jrnl_state_ctx s
     end.
 
+  Definition jrnl_crash_ctx {Σ} {jG: jrnlG Σ} : iProp Σ :=
+    ∃ m, ([∗ map] a ↦ v ∈ jrnlData m, jrnl_crash_tok a) ∗
+          map_ctx jrnlG_crash_toks_name 1 ((λ _, tt) <$> jrnlData m).
+
   Definition jrnl_state_start {Σ} {jG: jrnlG Σ} (m: jrnl_map) : iProp Σ :=
-    [∗ map] a ↦ v ∈ jrnlData m, jrnl_mapsto a 1 v.
+    ([∗ map] a ↦ v ∈ jrnlData m, jrnl_mapsto a 1 v) ∗
+    ([∗ map] a ↦ v ∈ jrnlData m, jrnl_crash_tok a).
+
+  Definition jrnl_state_restart {Σ} {jG: jrnlG Σ} (m: jrnl_map) : iProp Σ :=
+    ([∗ map] a ↦ v ∈ jrnlData m, jrnl_crash_tok a).
 
   Definition jrnl_start {Σ} {jG: jrnlG Σ} (jrnl: @ffi_state jrnl_model) : iProp Σ :=
     match jrnl with
@@ -277,8 +296,8 @@ Section jrnl_interp.
 
   Definition jrnl_restart {Σ} (jG: jrnlG Σ) (jrnl: @ffi_state jrnl_model) : iProp Σ :=
     match jrnl with
-    | Opened s => jrnl_open
-    | Closed s => jrnl_closed_frag
+    | Opened s => jrnl_open ∗ jrnl_state_restart s
+    | Closed s => jrnl_closed_frag ∗ jrnl_state_restart s
     end.
 
   Program Instance jrnl_interp : ffi_interp jrnl_model :=
@@ -379,14 +398,18 @@ Next Obligation.
   iMod (own_alloc (Cinl (1%Qp, to_agree tt) : openR)) as (γ1) "H".
   { repeat econstructor => //=. }
   iMod (map_init_many (jrnlData m)) as (γdata) "(Hdata_ctx&Hdata)".
+  iMod (map_init_many ((λ _, tt) <$> jrnlData m)) as (γcrash) "(Hcrash_ctx&Hcrash)".
   iMod (own_alloc (to_agree (jrnlKinds m : leibnizO (gmap blkno kind)))) as (γkinds) "#Hkinds".
   { constructor. }
-  iExists {| jrnl_names_open := γ1; jrnl_names_data := γdata; jrnl_names_kinds := γkinds |}.
+  iExists {| jrnl_names_open := γ1; jrnl_names_data := γdata; jrnl_names_kinds := γkinds;
+             jrnl_names_crash := γcrash |}.
   iFrame. iModIntro. iFrame "% #".
   rewrite assoc.
   iSplitL "H".
   { by rewrite -own_op -Cinl_op -pair_op frac_op Qp_half_half agree_idemp. }
   rewrite /jrnl_state_start.
+  rewrite big_sepM_fmap.
+  iFrame.
   iDestruct (big_sepM.big_sepM_mono_with_inv with "Hkinds Hdata") as "(_&$)".
   iIntros (a x Hlookup) "(#Hkinds&Hpt)". iFrame "Hkinds".
   rewrite /jrnl_mapsto.
@@ -410,24 +433,36 @@ Next Obligation.
     (* XXX: monad_inv should handle *)
     iMod (own_alloc (Cinl (1%Qp, to_agree tt) : openR)) as (γ1) "H".
     { repeat econstructor => //=. }
+    iMod (map_init_many ((λ _, tt) <$> jrnlData s)) as (γcrash) "(Hcrash_ctx&Hcrash)".
     iExists {| jrnl_names_open := γ1;
                jrnl_names_data := jrnl_names_data (jrnl_get_names _);
-               jrnl_names_kinds := jrnl_names_kinds (jrnl_get_names _) |}.
+               jrnl_names_kinds := jrnl_names_kinds (jrnl_get_names _) ;
+               jrnl_names_crash := γcrash |}.
     iDestruct "Hinterp" as "(?&?)". rewrite //=/jrnl_restart//=.
     iFrame. rewrite comm -assoc. iSplitL ""; first eauto.
     rewrite /jrnl_closed_auth/jrnl_closed_frag.
+    rewrite big_sepM_fmap.
+    rewrite /jrnl_state_restart.
+    rewrite /jrnl_crash_tok.
+    rewrite //=. iFrame.
     iModIntro. by rewrite -own_op -Cinl_op -pair_op frac_op Qp_half_half agree_idemp.
   - inversion Hcrash. subst. inversion H1. subst. inversion H3. subst.
     inversion H2. subst. inversion H4. subst.
     (* XXX: monad_inv should handle *)
     iMod (own_alloc (Cinl (1%Qp, to_agree tt) : openR)) as (γ1) "H".
     { repeat econstructor => //=. }
+    iMod (map_init_many ((λ _, tt) <$> jrnlData s)) as (γcrash) "(Hcrash_ctx&Hcrash)".
     iExists {| jrnl_names_open := γ1;
                jrnl_names_data := jrnl_names_data (jrnl_get_names _);
-               jrnl_names_kinds := jrnl_names_kinds (jrnl_get_names _) |}.
+               jrnl_names_kinds := jrnl_names_kinds (jrnl_get_names _) ;
+               jrnl_names_crash := γcrash |}.
     iDestruct "Hinterp" as "(?&?)". rewrite //=/jrnl_restart//=.
     iFrame. rewrite comm -assoc. iSplitL ""; first eauto.
     rewrite /jrnl_closed_auth/jrnl_closed_frag.
+    rewrite big_sepM_fmap.
+    rewrite /jrnl_state_restart.
+    rewrite /jrnl_crash_tok.
+    rewrite //=. iFrame.
     iModIntro. by rewrite -own_op -Cinl_op -pair_op frac_op Qp_half_half agree_idemp.
 Qed.
 
@@ -980,6 +1015,60 @@ Proof.
   { destruct Hwf as (?&?&?&?). eauto. }
   iMod ("Hclo" with "[Hσ Hrest H Hffi]") as "_".
   { iNext. iExists _. iFrame "H". iFrame. }
+  iModIntro. iFrame.
+Qed.
+
+Lemma ghost_step_jrnl_atomically_crash E j K {HCTX: LanguageCtx K} (l: sval) e σj (v: sval) σj' :
+  always_steps e σj v σj' →
+  nclose sN ⊆ E →
+  spec_crash_ctx (jrnl_crash_ctx) -∗
+  ([∗ map] a ↦ o ∈ (jrnlData σj), jrnl_mapsto a 1 o) -∗
+  ([∗ map] a ↦ _ ∈ (jrnlData σj), jrnl_crash_tok a) -∗
+  jrnl_kinds_lb (jrnlKinds σj) -∗
+  jrnl_open -∗
+  j ⤇ K (Atomically l e)
+  -∗ |C={E}_0=>
+    ([∗ map] a ↦ o ∈ (jrnlData σj'), jrnl_mapsto a 1 o) ∗
+    ([∗ map] a ↦ _ ∈ (jrnlData σj), jrnl_crash_tok a).
+Proof.
+  iIntros (Hsteps ?) "(#Hctx&#Hstate) Hσj_data Hσj_crash_toks Hσj_kinds Hopen Hj".
+  destruct Hsteps as (Heq_kinds&Hwf&Hrtc).
+  iMod (cfupd_weaken_all with "Hstate") as "#Hstate'"; eauto.
+  { solve_ndisj. }
+  iInv "Hstate'" as "[>Hbad|Hrest]" "Hclo".
+  { iIntros "HC".
+    destruct Hwf as (Hdom&?).
+    iDestruct "Hbad" as (?) "(Htok&Hcrash_ctx)".
+    induction (jrnlData σj) as [| x v' ? ? _] using map_ind.
+    { rewrite dom_empty_L in Hdom. symmetry in Hdom. apply dom_empty_inv_L in Hdom. rewrite Hdom.
+      rewrite ?big_sepM_empty. iMod ("Hclo" with "[-]").
+      { iLeft. iNext; iExists _; eauto. iFrame. }
+      eauto. }
+    iEval (rewrite big_sepM_insert //) in "Hσj_crash_toks".
+    iDestruct "Hσj_crash_toks" as "(Hcrash1&_)".
+    iDestruct (map_valid with "[$] Hcrash1") as %Hlookup.
+    apply lookup_fmap_Some in Hlookup as (?&_&Hlookup).
+    iDestruct (big_sepM_lookup_acc _ _ _ _ Hlookup with "Htok") as "(H1&_)"; eauto.
+    iDestruct (ptsto_conflict with "[$] [$]") as %[].
+  }
+  iDestruct "Hrest" as (s) "(>H&Hinterp)".
+  iDestruct "Hinterp" as "(>Hσ&>Hffi&?&?&?&>Hctok)".
+  iDestruct (jrnl_ctx_sub_state_valid with "[$] [$] [$] [$]") as %Hsub.
+  iIntros "HC".
+  iMod (ghost_step_crash_lifting _ _ _ _ _ (Atomically l e) s [] (jrnl_upd σj' s) (SOMEV v) []
+          with "[] Hctok Hj Hctx H HC") as "(Hctok&Hj&H&_)".
+  { apply head_prim_step.
+    apply head_step_atomically.
+    eapply Hrtc.
+    auto.
+  }
+  { solve_ndisj. }
+  { iModIntro. iIntros "(H1&>H2)". iDestruct (pending_pending with "[$] [$]") as %[]. }
+  iMod (jrnl_ctx_upd _ (jrnlData σj') with "[$] [$] [$] [$]") as "(Hσj'_data&Hffi)".
+  { destruct Hwf as (?&?&?&?). rewrite Heq_kinds; eauto. }
+  { destruct Hwf as (?&?&?&?). eauto. }
+  iMod ("Hclo" with "[-Hσj_crash_toks Hσj'_data]") as "_".
+  { iNext. iRight. iExists _. iFrame "H". iFrame. }
   iModIntro. iFrame.
 Qed.
 
